final project details

code.lisp
@@ -1,15 +1,21 @@
-; structure verifiers
+;;;;;;;;;;;;;;;;;;;;;;;;;;;;;
+; paths
 (defun pathp (p)
   (if (endp p)
       t
     (and (symbolp (car p))
          (pathp (cdr p)))))
 
+(defun inop (x)
+  (natp x))
+;;;;;;;;;;;;;;;;;;;;;;;;;;;;;
+; tree nodes
 (defun filep (x)
   (and (consp x)
        (equal (car x) :file)
        (consp (cdr x))
-       (null (cddr x))))
+       (null (cddr x))
+       (inop (cadr x))))
 
 (mutual-recursion
 
@@ -18,8 +24,10 @@
    (and (consp x)
         (equal (car x) :dir)
         (consp (cdr x))
-        (null (cddr x))
-        (entriesp (cadr x))))
+        (consp (cddr x))
+        (null (cdddr x))
+        (inop (cadr x))
+        (entriesp (caddr x))))
 
  (defun entryp (x)
    (declare (xargs :measure (acl2-count x)))
@@ -39,11 +47,46 @@
   (or (filep x)
       (dirp x)))
 
-(defun valid-fs (fs)
+(defun valid-tree (fs)
   (dirp fs))
+;;;;;;;;;;;;;;;;;;;;;;;;;;;;;;;;;;;
+; inodes
+(defun inodep (x)
+  (and (consp x)
+       (equal (car x) :inode)
+       (consp (cdr x))
+       (consp (cddr x))
+       (consp (cdddr x))
+       (consp (cddddr x))
+       (null (cdr (cddddr x)))
+       (inop (cadr x))
+       (or (equal (caddr x) :file)
+           (equal (caddr x) :dir))
+       (symbolp (cadddr x))
+       (natp (car (cddddr x)))))
 
+(defun inode-entry-p (x)
+  (and (consp x)
+       (inop (car x))
+       (inodep (cdr x))))
 
-; helper functions
+(defun inode-table-p (tbl)
+  (if (endp tbl)
+      t
+    (and (inode-entry-p (car tbl))
+         (inode-table-p (cdr tbl)))))
+;;;;;;;;;;;;;;;;;;;;;;;;;;;;;;;;;
+; whole file system !
+(defun hfs-p (x)
+  (and (consp x)
+       (equal (car x) :fs)
+       (consp (cdr x))
+       (consp (cddr x))
+       (null (cdddr x))
+       (valid-tree (cadr x))
+       (inode-table-p (caddr x))))
+;;;;;;;;;;;;;;;;;;;;;;;;;;;;;;;;;
+; tree helpers
 (defun lookup-name (name entries)
   (if (endp entries)
       nil
@@ -60,35 +103,173 @@
       (cons (car entries)
             (put-name name node (cdr entries))))))
 
+(defun remove-name (name entries)
+  (if (endp entries)
+      nil
+    (if (equal name (caar entries))
+        (cdr entries)
+      (cons (car entries)
+            (remove-name name (cdr entries))))))
 
-; filesystem operations
-(defun lookup-path (p fs)
+(defun node-ino (node)
+  (if (filep node)
+      (cadr node)
+    (if (dirp node)
+        (cadr node)
+      nil)))
+;;;;;;;;;;;;;;;;;;;;;;;;;;;;;;;;;;;;;;;;;;;;;;;;
+; inode table helpers
+(defun lookup-inode (ino tbl)
+  (if (endp tbl)
+      nil
+    (if (equal ino (caar tbl))
+        (cdar tbl)
+      (lookup-inode ino (cdr tbl)))))
+
+(defun put-inode (ino inode tbl)
+  (if (endp tbl)
+      (list (cons ino inode))
+    (if (equal ino (caar tbl))
+        (cons (cons ino inode)
+              (cdr tbl))
+      (cons (car tbl)
+            (put-inode ino inode (cdr tbl))))))
+
+(defun remove-inode (ino tbl)
+  (if (endp tbl)
+      nil
+    (if (equal ino (caar tbl))
+        (cdr tbl)
+      (cons (car tbl)
+            (remove-inode ino (cdr tbl))))))
+
+(defun remove-inode-list (inos tbl)
+  (if (endp inos)
+      tbl
+    (remove-inode-list (cdr inos)
+                       (remove-inode (car inos) tbl))))
+;;;;;;;;;;;;;;;;;;;;;;;;;;;;;;;;;;;;;;;;;;;;;;;;
+; lookup
+(defun lookup-path-tree (p fs)
   (if (endp p)
       fs
     (if (dirp fs)
-        (lookup-path (cdr p)
-                     (lookup-name (car p) (cadr fs)))
+        (lookup-path-tree (cdr p)
+                          (lookup-name (car p) (caddr fs)))
       nil)))
 
-(defun insert-path (p name newnode fs)
+(defun lookup-path (p hfs)
+  (if (hfs-p hfs)
+      (lookup-path-tree p (cadr hfs))
+    nil))
+
+(defun lookup-path-inode (p hfs)
+  (let ((node (lookup-path p hfs)))
+    (if (and (hfs-p hfs)
+             (nodep node))
+        (lookup-inode (node-ino node)
+                      (caddr hfs))
+      nil)))
+;;;;;;;;;;;;;;;;;;;;;;;;;;;;;;;;;;;;;;;;;;;;;;;;
+; insert and delete path tree
+(defun insert-path-tree (p name newnode fs)
   (if (not (dirp fs))
       fs
     (if (endp p)
         (list :dir
-              (put-name name newnode (cadr fs)))
-      (let ((child (lookup-name (car p) (cadr fs))))
+              (cadr fs)
+              (put-name name newnode (caddr fs)))
+      (let ((child (lookup-name (car p) (caddr fs))))
         (if (dirp child)
             (list :dir
+                  (cadr fs)
                   (put-name (car p)
-                            (insert-path (cdr p) name newnode child)
-                            (cadr fs)))
+                            (insert-path-tree (cdr p) name newnode child)
+                            (caddr fs)))
           fs)))))
 
-; theorem
-(defthm final-project
-  (implies (and (valid-fs fs)
+(defun delete-path-tree (p name fs)
+  (if (not (dirp fs))
+      fs
+    (if (endp p)
+        (list :dir
+              (cadr fs)
+              (remove-name name (caddr fs)))
+      (let ((child (lookup-name (car p) (caddr fs))))
+        (if (dirp child)
+            (list :dir
+                  (cadr fs)
+                  (put-name (car p)
+                            (delete-path-tree (cdr p) name child)
+                            (caddr fs)))
+          fs)))))
+
+;;;;;;;;;;;;;;;;;;;;;;;;;;;;;;;;
+; collect inode numbers in a subtree
+(mutual-recursion
+
+ (defun collect-inos-node (node)
+   (declare (xargs :measure (acl2-count node)))
+   (if (filep node)
+       (list (cadr node))
+     (if (dirp node)
+         (cons (cadr node)
+               (collect-inos-entries (caddr node)))
+       nil)))
+
+ (defun collect-inos-entries (entries)
+   (declare (xargs :measure (acl2-count entries)))
+   (if (endp entries)
+       nil
+     (append (collect-inos-node (cdar entries))
+             (collect-inos-entries (cdr entries))))))
+
+;;;;;;;;;;;;;;;;;;;;;;;;;;;;;;;;;;;;;
+; insert and delete path
+(defun insert-path (p name newnode newinode hfs)
+  (if (not (hfs-p hfs))
+      hfs
+    (let ((newtree (insert-path-tree p name newnode (cadr hfs))))
+      (if (equal newtree (cadr hfs))
+          hfs
+        (list :fs
+              newtree
+              (put-inode (node-ino newnode)
+                         newinode
+                         (caddr hfs)))))))
+
+(defun delete-path (p name hfs)
+  (if (not (hfs-p hfs))
+      hfs
+    (let* ((victim (lookup-path-tree (append p (list name)) (cadr hfs)))
+           (newtree (delete-path-tree p name (cadr hfs)))
+           (inos-to-remove (collect-inos-node victim))
+           (newtbl (remove-inode-list inos-to-remove (caddr hfs))))
+      (list :fs newtree newtbl))))
+
+; theorems
+(defthm insert-path-preserves-or-updates-inode-table
+  (implies (and (hfs-p hfs)
                 (pathp p)
                 (symbolp name)
-                (nodep v))
-           (valid-fs (insert-path p name v fs)))
-  :instructions (:prove))
+                (nodep newnode)
+                (inodep newinode))
+           (or (equal (caddr (insert-path p name newnode newinode hfs))
+                      (caddr hfs))
+               (equal (caddr (insert-path p name newnode newinode hfs))
+                      (put-inode (node-ino newnode)
+                                 newinode
+                                 (caddr hfs))))))
+(defthm delete-path-updates-inode-table
+  (implies (and (hfs-p hfs)
+                (pathp p)
+                (symbolp name))
+           (or (equal (caddr (delete-path p name hfs))
+                      (caddr hfs))
+               (equal (caddr (delete-path p name hfs))
+                      (remove-inode-list
+                       (collect-inos-node
+                        (lookup-path-tree (append p (list name))
+                                          (cadr hfs)))
+                       (caddr hfs))))))
+
